src/named/PfCore.v
@@ -12,6 +12,19 @@ Import OptionMonad.
 Require Import String.
 
 
+(*TODO: where is the right place for these? Utils rewrite base?*)
+Hint Rewrite in_cons : utils.
+Hint Rewrite pair_equal_spec : utils.
+
+(*TODO: mvoe to Utils *)
+(*TODO: put in utils, add nil lemma *)
+Lemma fresh_cons A n m (e:A) es : fresh n ((m,e)::es) <-> (~ n = m) /\ fresh n es.
+Proof.
+  repeat (simpl in *; autorewrite with bool_utils utils in * ); intuition auto.
+Qed.
+Hint Rewrite fresh_cons : utils.
+Arguments fresh : simpl never.
+
 (*TODO: move to utils/rewriting package*)
 Lemma invert_list_Forall_nil A (P : A -> Prop)
   : List.Forall P [::] <-> True.
@@ -26,1789 +39,216 @@ Proof.
   safe_invert H; auto.  
 Qed.
 Hint Rewrite invert_list_Forall_cons : utils.
-
-(*TODO: pull/duplicate appropriate hints outside the section*)
-Section TermsAndRules.
-  Context (l : wfexp_lang).
-  Context (l_ok : wf_lang l).
-
   
-  Lemma wf_lang_all_fresh : all_fresh l.
-  Proof.
-    revert l_ok; induction l; break; simpl in *;
-      intro H; inversion H; subst; break_goal; auto.
-  Qed.
-  Hint Resolve wf_lang_all_fresh : pfcore.
-
-  (*
-  
-  (*
-    Congruence lemmas for rewriting
-    TODO: go in Pf?
-   *)
-  Lemma pvar_cong x y : pvar x = pvar y <-> x = y.
-  Proof.
-    intuition; inversion H; eauto with pfcore.
-  Qed.
-  Hint Rewrite pvar_cong : pfcore.
-  Lemma pcon_cong n1 n2 pl1 pl2 : pcon n1 pl1 = pcon n2 pl2 <-> (n1 = n2 /\ pl1 = pl2).
-  Proof.
-    intuition; subst; try inversion H; eauto with pfcore.
-  Qed.
-  Hint Rewrite pcon_cong : pfcore.
-    
-  (*Inversion lemmas for rewriting is_dom and is_codom
-    when we know the top-level structure of their arguments
-   *)
-  Lemma invert_is_dom_var x p : is_dom (pvar x) p <-> p = pvar x.
-  Proof.
-    split; [intro H; inversion H| intros; subst];
-      eauto with pfcore.
-  Qed.
-  Hint Rewrite invert_is_dom_var : pfcore.
-  Lemma invert_is_dom_con n1 p pl
-    : is_dom (pcon n1 pl) p
-      <-> (exists pl_r, (List.Forall2 is_dom pl pl_r) /\ p = pcon n1 pl_r).
-  Proof.
-    split.
-    - intro H; inversion H; eauto with pfcore.
-    - firstorder; subst; eauto with pfcore.
-  Qed.
-  Hint Rewrite invert_is_dom_con : pfcore.
-  
-  Lemma invert_is_dom_ax n pfs p'
-    : is_dom (ax n pfs) p' <->
-      (exists r, (n,r) \in l /\ 
-                 match r with
-                 | sort_le_pf c p _
-                 | term_le_pf c p _ _ =>
-                   exists pl_r, List.Forall2 is_dom pfs pl_r /\
-                                p' = pf_subst (with_names_from c pl_r) p
-                 | _ => False
-                 end).
-  Proof.
-    split.
-    - intro H; inversion H; subst;
-      match goal with [H : is_true((_, ?r) \in _)|-_] =>
-                        exists r
-        end; eauto with pfcore.
-    - move => [r [rin ]].
-      destruct r; cbn; try easy;
-      move => [pl_r [ peq fall]]; subst; eauto with pfcore.
-  Qed.
-  Hint Rewrite invert_is_dom_ax : pfcore.
-  
-  Lemma invert_is_dom_sym p p' : is_dom (sym p) p' <-> is_codom p p'.
-  Proof.
-    split; [intro H; inversion H| intros; subst];
-      eauto with pfcore.
-  Qed.
-  Hint Rewrite invert_is_dom_sym : pfcore.
-  
-  Lemma invert_is_dom_trans p1 p2 p' : is_dom (trans p1 p2) p' <-> is_dom p1 p'.
-  Proof.
-    split; [intro H; inversion H| intros; subst];
-      eauto with pfcore.
-  Qed.
-  Hint Rewrite invert_is_dom_trans : pfcore.
-  
-  Lemma invert_is_dom_conv pt p p'
-    : is_dom (conv pt p) p' <->
-      exists p'', is_dom p p'' /\ p' = (conv pt p'') .
-  Proof.
-    split; [intro H; inversion H| intros; subst];
-      firstorder; subst;
-      eauto with pfcore.
-  Qed.
-  Hint Rewrite invert_is_dom_conv : pfcore.
-
-  Lemma invert_is_codom_var x p : is_codom (pvar x) p <-> p = pvar x.
-  Proof.
-    split; [intro H; inversion H| intros; subst];
-      eauto with pfcore.
-  Qed.
-  Hint Rewrite invert_is_codom_var : pfcore.
-  Lemma invert_is_codom_con n1 p pl
-    : is_codom (pcon n1 pl) p
-      <-> exists pl_r, List.Forall2 is_codom pl pl_r /\ p = pcon n1 pl_r.
-  Proof.
-    split.
-    - intro H; inversion H; eauto with pfcore.
-    - firstorder; subst; eauto with pfcore.
-  Qed.
-  Hint Rewrite invert_is_codom_con : pfcore.
-  
-  Lemma invert_is_codom_ax n pfs p'
-    : is_codom (ax n pfs) p' <->
-      (exists r, (n,r) \in l /\ 
-                 match r with
-                 | sort_le_pf c _ p
-                 | term_le_pf c _ p _ =>
-                   exists pl_r, List.Forall2 is_codom pfs pl_r /\
-                                p' = pf_subst (with_names_from c pl_r) p                                
-                 | _ => False
-                 end).
-  Proof.
-    split.
-    - intro H; inversion H; subst;
-      match goal with [H : is_true((_, ?r) \in _)|-_] =>
-                        exists r
-        end; eauto with pfcore.
-    - move => [r [rin ]].
-      destruct r; cbn; try easy;
-      move => [pl_r [ peq fall]]; subst; eauto with pfcore.
-  Qed.
-  Hint Rewrite invert_is_codom_ax : pfcore.
-
-  Lemma invert_is_codom_sym p p' : is_codom (sym p) p' <-> is_dom p p'.
-  Proof.
-    split; [intro H; inversion H| intros; subst];
-      eauto with pfcore.
-  Qed.
-  Hint Rewrite invert_is_codom_sym : pfcore.
-  
-  Lemma invert_is_codom_trans p1 p2 p' : is_codom (trans p1 p2) p' <-> is_codom p2 p'.
-  Proof.
-    split; [intro H; inversion H| intros; subst];
-      eauto with pfcore.
-  Qed.
-  Hint Rewrite invert_is_codom_trans : pfcore.
-  
-  Lemma invert_is_codom_conv pt p p'
-    : is_codom (conv pt p) p' <->
-      exists p'', is_codom p p'' /\ p' = (conv pt p'').
-  Proof.
-    split; [intro H; inversion H| intros; subst];
-      firstorder; subst;
-      eauto with pfcore.
-  Qed.
-  Hint Rewrite invert_is_codom_conv : pfcore.
-
-
-  (*We want this as a lemma so it can be part of autorewrite
-    instead of using both autorewrite and cbn
-   *)
-  Lemma omap_eval_Some (A B:eqType) (f : A -> B) a
-    : omap f (Some a) = Some (f a).
-  Proof. reflexivity. Qed.
-  Hint Rewrite omap_eval_Some : utils.
-  
-  Lemma omap_eval_None (A B:eqType) (f : A -> B)
-    : omap f None = None.
-  Proof. reflexivity. Qed.
-  Hint Rewrite omap_eval_None : utils.
-
-
-  Ltac prepare_crush :=
-    repeat(autorewrite with utils bool_utils pfcore in *;
-           try match goal with
-           | [H : exists _,_|- _] => destruct H
-           | [H : _ /\ _ |- _] => destruct H
-           end;
-           subst).
-  
-  (*TODO: separate inversion database,
-    custom plugin to greedily run database?
-    Or: inversion lemmas, rewriting
-   *)
-  Hint Extern 1 => match goal with [H : is_dom _ _|-_] => safe_invert H end : pfcore.
-  Hint Extern 1 => match goal with [H : is_codom _ _|-_] => safe_invert H end : pfcore.
-  Hint Extern 1 => match goal with [H : List.Forall2 _ _ _|-_] => safe_invert H end : pfcore.
-  Hint Extern 1 => match goal with [H : Some _ = None|-_] => safe_invert H end : pfcore.
-  Hint Extern 1 => match goal with [H : None = Some _|-_] => safe_invert H end : pfcore.
-  Hint Extern 1 => match goal with [H : Some _ = Some _|-_] => safe_invert H end : pfcore.
-  Hint Extern 1 => match goal with [H : omap _ ?e = Some _|-_] => let H:=fresh in my_case H e;
-                prepare_crush end : pfcore.
-
-  (*
-  Hint Extern 2 (reflect _ (omap _ ?e == _)) =>
-  (let H:= fresh in my_case H e; prepare_crush) : pfcore.
-  Hint Extern 4 (reflect _ (_ == _)) =>
-  (destruct_reflect_bool; prepare_crush) : pfcore.
-   *)
-  (*TODO: move to utils*)
-  (*
-  Hint Extern 10 => match goal with
-                    |[H : forall x, reflect (?A x) _ |- ?A _] =>
-                      apply /H; prepare_crush
-                    |[H : reflect ?A _ |- ?A] =>
-                      apply /H; prepare_crush
-                    end : bool_utils.
-  Hint Extern 10 => match goal with
-                    | [H : forall x, reflect (?A x) _, H': ?A _ |-_] =>
-                      move: H' => /H H'; prepare_crush
-                    | [H : reflect ?A _, H':?A|-_] =>
-                      move: H' => /H H'; prepare_crush
-                    end : bool_utils.
-   *)
-  
-  Lemma dom_args_eval_cons p ps
-    : dom_args dom (p :: ps) = do l_dom <- dom_args dom ps; a_dom <- dom p; ret (a_dom::l_dom).
-  Proof.
-    reflexivity.
-  Qed.
-  Hint Rewrite dom_args_eval_cons : pfcore.  
-  Lemma codom_args_eval_cons p ps
-    : codom_args codom (p :: ps) = do l_codom <- codom_args codom ps; a_codom <- codom p; ret (a_codom::l_codom).
-  Proof.
-    reflexivity.
-  Qed.
-  Hint Rewrite codom_args_eval_cons : pfcore.
-
-  
-  Hint Rewrite @named_list_lookup_err_inb : pfcore.
-  Lemma named_list_lookup_err_inb' (A:eqType)
-    : forall (l0 : named_list A) (x : string) (v : A),
-      all_fresh l0 ->
-      (named_list_lookup_err l0 x = Some v) <-> ((x, v) \in l0).
-  Proof.
-    intros; rewrite <- named_list_lookup_err_inb; auto.
-    split.
-    move => -> //.
-    move => /eqP //.
-  Qed.    
-  Hint Rewrite named_list_lookup_err_inb' : pfcore.
-
-  
-  Hint Extern 4 False =>
-  match goal with
-    [ H_fr : is_true(all_fresh ?l),
-             H : is_true((?n, ?a) \in ?l),
-                 H' : is_true((?n, ?b) \in ?l)
-      |-_]=>
-    let Heq := fresh in
-    assert(a = b) as Heq; [ eapply in_all_fresh_same; solve[eauto]| safe_invert Heq]
-  end : pfcore.
-
-  
-  Hint Extern 1 (~ is_dom (ax _ _) _) => let H := fresh in intro H; inversion H; clear H; subst : pfcore.
-  
-  Ltac crush_n n := prepare_crush; eauto n with pfcore bool_utils.
-  Ltac crush := crush_n integer:(5).
-
-
-  Lemma lookup_is_exp pl x
-    :List.Forall (fun p => is_exp p) (map snd pl) ->
-     is_exp (named_list_lookup (pvar x) pl x).
-  Proof.
-    induction pl; break; simpl in *; crush.
-    case_match; crush; intuition.
-  Qed.
-    
-  Lemma subst_is_exp p pl
-    : is_exp p ->
-      List.Forall (fun p=> is_exp p) (map snd pl) ->
-      is_exp (pf_subst pl p).
-  Proof.
-    induction p; simpl; crush.
-    {
-        intros; by apply lookup_is_exp.
-    }
-    {
-      revert dependent l0;
-        induction l0;
-        simpl; crush;
-          intuition.
-    }
-  Qed.
-  Hint Resolve subst_is_exp : pfcore.
-
-  
-  Lemma sort_le_in_left_is_exp n c p p_r
-    : (n, sort_le_pf c p p_r)\in l -> is_exp p.
-  Proof.
-    induction l_ok; simpl; try easy.
-    rewrite in_cons.
-    move => /orP [/eqP []|]; intros; subst; eauto.
-      by inversion H0.
-  Qed.
-  
-  Lemma sort_le_in_right_is_exp n c p p_l
-    : (n, sort_le_pf c p_l p)\in l -> is_exp p.
-  Proof.
-    induction l_ok; simpl; try easy.
-    rewrite in_cons.
-    move => /orP [/eqP []|]; intros; subst; eauto.
-      by inversion H0.
-  Qed.
-    
-  Lemma term_le_in_left_is_exp n c p p_r t
-    : (n, term_le_pf c p p_r t)\in l -> is_exp p.
-  Proof.
-    induction l_ok; simpl; try easy.
-    rewrite in_cons.
-    move => /orP [/eqP []|]; intros; subst; eauto.
-      by inversion H0.
-  Qed.
-    
-  Lemma term_le_in_right_is_exp n c p_l p t
-    : (n, term_le_pf c p_l p t)\in l -> is_exp p.
-  Proof.
-    induction l_ok; simpl; try easy.
-    rewrite in_cons.
-    move => /orP [/eqP []|]; intros; subst; eauto.
-      by inversion H0.
-  Qed.
-
-  
-  (*TODO: move to utils/rewriting package*)
-  (*TODO: leave generic in second arg or no*)
-  Lemma invert_list_Forall2_nil A B (P : A -> B -> Prop) es
-    : List.Forall2 P [::] es <-> es = [::].
-  Proof.
-    intuition; subst; auto.
-  Qed.
-  Hint Rewrite invert_list_Forall2_nil : utils.
-  Lemma invert_list_Forall2_cons A B (P : A -> B -> Prop) e es lst
-    : List.Forall2 P (e::es) lst <->
-      exists es', List.Forall2 P es es' /\
-      exists e', P e e' /\ lst = e'::es'.
-  Proof.
-    intuition;
-      safe_invert H; firstorder; subst; auto.  
-  Qed.
-  Hint Rewrite invert_list_Forall2_cons : utils.
-
-  Lemma invert_cons_eq A (a a':A) lst lst'
-    : a::lst = a' ::lst' <-> a = a' /\ lst = lst'.
-  Proof.
-    intuition; try safe_invert H; firstorder; subst; auto.
-  Qed.
-  Hint Rewrite invert_cons_eq : utils.
-      
-  Lemma dom_codom_is_exp p
-    : (forall p', is_dom p p' -> is_exp p')
-      /\ (forall p', is_codom p p' -> is_exp p').
-  Proof.
-    induction p; split; intros; crush.
-    1,2:revert dependent l0; intro l0; revert x;
-        induction l0; firstorder; crush.
-    1,2:  destruct x; simpl in *; intuition; crush;
-      apply subst_is_exp;
-        eauto using
-              sort_le_in_left_is_exp,
-        term_le_in_left_is_exp,
-        term_le_in_right_is_exp,
-        sort_le_in_right_is_exp;
-      clear H0;
-      revert dependent pfs; intro l0; revert n0 x;
-        induction l0; intros; destruct n0; break;
-          destruct x as [|? x];
-          simpl in *; crush; try easy.
-  Qed.
-
-  Definition dom_is_exp p := proj1 (dom_codom_is_exp p).
-  Hint Resolve dom_is_exp : pfcore.
-  Definition codom_is_exp p := proj2 (dom_codom_is_exp p).
-  Hint Resolve codom_is_exp : pfcore.
-   
-  Lemma exists_pcon_eq s pl s' P
-    : (exists pl', pcon s pl = pcon s' pl' /\ P pl')
-      <-> (s = s' /\ P pl).
-  Proof.
-    firstorder; inversion H; eauto with pfcore.
-  Qed.
-  Hint Rewrite exists_pcon_eq : pfcore.
-
-  
-  Lemma invert_Forall2_cons (A B : eqType) R (e : A) es (e' : B) es'
-    : List.Forall2 R (e::es) (e'::es') <-> (R e e' /\ List.Forall2 R es es').
-  Proof.
-    split; intuition.
-  Qed.
-  Hint Rewrite invert_Forall2_cons : utils.
-
-  (*
-  (*TODO: need to recover level of indirection;
-   what is the best way? make use of hint resolve not rewrite
-   *)
-  Lemma exists_as_omap_eq (A B:eqType) P (f : A -> B) a b
-    : (forall c, P c <-> b = Some c) ->
-      (exists c : A, a = f c /\ P c) <-> omap f b = Some a.
-  Proof.
-    destruct b; cbn; firstorder; crush; firstorder.
-    specialize (H x); firstorder; crush.
-    exists s.
-    specialize (H s); firstorder; crush.
-    specialize (H x); firstorder; crush.
-  Qed.
-  Hint Resolve exists_as_omap_eq : pfcore.
-*)
-
-  (*
-  Lemma exists_as_obind_eq (A B:eqType) P Q (f : A -> option B) a b
-    : (forall c, P c <-> b = Some c) ->
-      (forall c, Q c <-> f c = Some a) ->
-      (exists c, P c /\ Q c) <-> obind f b = Some a.
-  Proof.
-    my_case beq b; cbn; firstorder; crush;
-    specialize (H x); specialize (H0 x); firstorder; crush.
-  Qed.
-  Hint Resolve exists_as_obind_eq : pfcore.
-*)
-
-  (*
-  Ltac fold_omap :=
-    lazymatch goal with
-      [|- context c[match ?e with Some p => Some (@?f p) | None => None end] ]=>
-      let g := context c [omap f e] in
-      change g
-    end.
-
-  
-  Ltac fold_obind :=
-    lazymatch goal with
-      [|- context c[match ?e with Some p => (@?f p) | None => None end] ]=>
-      let g := context c [obind f e] in
-      change g
-    end.
-    *)
-  (*
-  Lemma rewrite_pair_exists A B P
-    : (exists (a:A) (b: B), P a b) <-> exists (p : A * B), P p.1 p.2.
-  Proof.
-    firstorder.
-    exists (x,x0); simpl; auto.
-  Qed.
-  Hint Rewrite rewrite_pair_exists : utils. *)
-
-  (*
-  Lemma rewrite_exists_match_cons (A:eqType) (Q : A -> _ -> Prop) x
-    : (exists a b, x = a::b /\ Q a b) <-> match x with
-                                          | [::] => False
-                                          | a::b => Q a b
-                                          end.
-  Proof.
-    destruct x; simpl; firstorder; safe_invert H; auto.
-  Qed.
-   *)
-
-
-  (*TODO: go back to all rules, review;
-    want to rewrite computations to props
-   *)
-  Lemma match_some_eq (A B: eqType) (ma : option A) f (b :B)
-    : match ma with Some a => f a | None => None end = Some b
-      <-> match ma with Some a => f a = Some b | None => False end.
-  Proof.
-    destruct ma; intuition; crush.
-  Qed.
-  Hint Rewrite match_some_eq : pfcore.
-  
-  Lemma some_to_exists_equal A (ma : option A) P
-    : match ma with
-      | Some e => P e
-      | None => False
-      end
-      <-> (exists e, ma = Some e /\ P e).
-  Proof.
-    destruct ma; simpl; firstorder; crush.
-  Qed.
-  Hint Rewrite some_to_exists_equal : pfcore.
-
-  
-  Lemma list_to_exists_equal A (ma : list A) P
-    : match ma with
-      | e::es => P e es
-      | [::] => False
-      end
-      <-> (exists e es, ma = e::es /\ P e es).
-  Proof.
-    destruct ma; simpl; firstorder; crush.
-    inversion H.
-  Qed.
-  Hint Rewrite list_to_exists_equal : pfcore.
-
-  
-  
-  Lemma rewrite_pair_let_to_proj A B (p : A*B) (P : A -> B -> Prop)
-    : (let (a,b) := p in P a b)
-      <-> P p.1 p.2 .
-  Proof.
-    destruct p; simpl; firstorder; crush.
-  Qed.
-  Hint Rewrite rewrite_pair_let_to_proj : pfcore.
-
-
-
-  
-  Ltac safe_specialize :=
-    match goal with
-      [ H : forall x, ?A -> _, H' : ?A|-_] =>
-      let H1 := fresh in
-      rename H into H1;
-        pose proof (fun x => H1 x H') as H;
-        clear H1
-    end.
-
-  Hint Extern 20 => match goal with
-       [ H : forall x, _ <-> _ |- _] =>
-       rewrite !H
-     end : bool_utils.
-
-  Local Lemma domP_inner_induction l0 l2
-    : List.fold_right
-        (fun t : pf =>
-           and ((forall p' : pf, (dom t = Some p') <-> (is_dom t p')) /\
-                 forall p' : pf, (codom t = Some p') <-> (is_codom t p'))) True
-        l0 ->
-      (dom_args dom l0 = Some l2) <->
-      (List.Forall2 is_dom l0 l2).
-  Proof.
-    revert l2; induction l0; cbn; intros; prepare_crush; repeat safe_specialize; crush.
-    apply peel_exists_iff; intro; crush.
-    apply and_iff_compat; crush.
-    apply peel_exists_iff; intro; crush.
-  Qed.
-  Hint Rewrite domP_inner_induction : pfcore.
-  
-   Local Lemma codomP_inner_induction l0 l2
-    : List.fold_right
-        (fun t : pf =>
-           and ((forall p' : pf, (dom t = Some p') <-> (is_dom t p')) /\
-                 forall p' : pf, (codom t = Some p') <-> (is_codom t p'))) True
-        l0 ->
-      (codom_args codom l0 = Some l2) <->
-      (List.Forall2 is_codom l0 l2).
-  Proof.
-    revert l2; induction l0; cbn; intros; prepare_crush; repeat safe_specialize; crush.
-    apply peel_exists_iff; intro; crush.
-    apply and_iff_compat; crush.
-    apply peel_exists_iff; intro; crush.
-  Qed.
-  Hint Rewrite codomP_inner_induction : pfcore.
- 
-  Lemma omap_eq_some A B (f : A -> B) ma b
-    : injective f ->
-      omap f ma = Some b <-> exists a, ma = Some a /\ f a = b.
-  Proof.
-    intro injf.
-    destruct ma; simpl; intuition; crush.
-  Qed.
-  Hint Rewrite omap_eq_some : pfcore.
-
-
-  Ltac injective_constructor :=
-    let H := fresh in intros ? ? H; safe_invert H; reflexivity.
-
-  
-  Hint Extern 1 (injective _) => injective_constructor : pfcore.
-
-  Lemma rewrite_none_eq_some A (a :A)
-    : None = Some a <-> False.
-  Proof.
-    intuition.
-  Qed.
-  Hint Rewrite rewrite_none_eq_some : pfcore.
-   
-  Lemma dom_codomP p
-    :(forall p', (dom p = Some p') <-> (is_dom p p'))
-       /\ (forall p', (codom p = Some p') <-> (is_codom p p')).
-  Proof.
-    induction p; split; cbn [dom codom]; fold dom; fold codom; intros;
-      crush;
-      try match goal with
-        [H : forall p', ?P p' <-> _ |- ?P _ <-> _] =>
-        rewrite H; crush
-          end;
-      (*TODO: why not auto?*)
-      apply peel_exists_iff; intro; crush.
-    all: apply and_iff_compat; crush.
-    all: destruct e; crush.
-    
-    all: apply peel_exists_iff; intro; crush.
-  Qed.
-
-  Definition rewrite_dom_eq p := proj1 (dom_codomP p).
-  Hint Rewrite rewrite_dom_eq : pfcore.
-  Definition rewrite_codom_eq p := proj2 (dom_codomP p).
-  Hint Rewrite rewrite_codom_eq : pfcore.
-
-    
-  Lemma is_domP p p' : reflect (is_dom p p') (dom p == Some p').
-  Proof.
-    eapply rewrite_reflect.
-    rewrite <- rewrite_dom_eq.
-    apply iff_refl.
-    apply eqP.
-  Qed.
-  Definition is_codomP p p' : reflect (is_codom p p') (codom p == Some p').
-  Proof.
-    eapply rewrite_reflect.
-    rewrite <- rewrite_codom_eq.
-    apply iff_refl.
-    apply eqP.
-  Qed.  
-      
-  (*TODO: relate dom to is_dom on ok terms
-    TODO: should dom be partial?
-    prob. want Inhabited typeclass first,
-    maybe this one too:
-    Class SyntaxWithPredicate t :=
-    {
-      inhabited :> Inhabited t;
-      is_ok : t -> Prop
-    }
-   *)
- 
-
-  
-  Lemma invert_term_ok_var c x t : term_ok l c (pvar x) t <-> (x,t) \in c.
-  Proof.
-    split; [intro H; inversion H| intros; subst];
-      eauto with pfcore.
-  Qed.
-  Hint Rewrite invert_term_ok_var : pfcore.
-  Lemma invert_sort_ok_var c x : sort_ok l c (pvar x) <-> False.
-  Proof.
-    split; [intro H; inversion H| intros; subst];
-      eauto with pfcore; easy.
-  Qed.
-  Hint Rewrite invert_sort_ok_var : pfcore.
-
-  Lemma invert_term_ok_con c n pl t
-    : term_ok l c (pcon n pl) t <->
-      exists r, (n,r) \in l /\
-      match r with
-      | term_rule_pf c' args t' =>
-        is_dom (pf_subst (with_names_from c' pl) t') t /\
-        args_ok l c pl c'
-      | _ => False
-      end.
-  Proof.
-    split; [intro H; inversion H| intros];
-      crush.
-    {
-      exists (term_rule_pf c' args t0); cbn;
-        intuition; crush.
-    }
-    {
-      destruct x; cbn in *; crush.
-    }
-  Qed.
-  Hint Rewrite invert_term_ok_con : pfcore.
-  
-  Lemma invert_sort_ok_con c n pl
-    : sort_ok l c (pcon n pl) <->
-      exists r, (n,r) \in l /\
-      match r with
-      | sort_rule_pf c' args =>
-        args_ok l c pl c'
-      | _ => False
-      end.
-  Proof.
-    split; [intro H; inversion H| intros];
-      intuition crush.
-    destruct x; crush.
-  Qed.
-  Hint Rewrite invert_sort_ok_con : pfcore.
-
-  Hint Resolve idP : bool_utils.
-
-  
-  Lemma invert_args_ok_nil c c'
-    : args_ok l c [::] c' <-> c' = [::].
-  Proof.
-    intuition crush.
-    safe_invert H; crush.
-  Qed.
-  Hint Rewrite invert_args_ok_nil : pfcore.
-
-  (*TODO: handle cases on snd arg?*)
-  Lemma invert_args_ok_cons c a pl c'
-    : args_ok l c (a::pl) c' <->
-      exists p c'', c' = p::c'' /\
-      exists t', is_dom (pf_subst (with_names_from c'' pl) p.2) t' /\
-                 term_ok l c a t' /\ args_ok l c pl c''.
-  Proof.
-    split; [intro H; inversion H| intros; subst]; firstorder; crush.
-    {
-      exists (name,t).
-      exists c'0.
-      split; crush.
-    }
-    {
-      destruct x; simpl in *; econstructor; crush.
-    }
-  Qed.
-  Hint Rewrite invert_args_ok_cons : pfcore.
-
-  
-  Lemma is_true_match_some A (ma : option A) f b
-    : is_true(match ma with Some a => f a | None => b end)
-      = match ma with Some a => is_true (f a) | None => is_true b end.
-  Proof.
-    destruct ma; reflexivity.
-  Qed.
-  Hint Rewrite is_true_match_some : bool_utils.
-
-  
-  Lemma is_true_match_list A (ma : list A) f b
-    : is_true(match ma with | a::ma' => f a ma' | [::] => b end)
-      = match ma with | a::ma' => is_true (f a ma') | [::] => is_true b end.
-  Proof.
-    destruct ma; reflexivity.
-  Qed.
-  Hint Rewrite is_true_match_list : bool_utils.
-
-
-  
-  Lemma rewrite_cons_eq_nil A (a : A) lst
-    : a::lst = [::] <-> False.
-  Proof.
-    intuition; inversion H.
-  Qed.
-  Hint Rewrite rewrite_cons_eq_nil : bool_utils.
-
-  (*A hack to get around rewrites that aren't working
-    under the match
-   *)
-  Lemma TMP_match_list_to_bool A (P : A -> list A -> Prop) c'
-    : match c' with
-      | [::] => false
-      | a0 :: ma' => P a0 ma'
-      end <->
-      match c' with
-      | [::] => False
-      | a0 :: ma' => P a0 ma'
-      end.
-  Proof.
-    destruct c'; simpl; crush.
-  Qed.
-
-  
-  Lemma TMP_match_option_to_bool A (P : A -> Prop) c'
-    : match c' with
-      | None => false
-      | Some a0 => P a0
-      end <->
-      match c' with
-      | None => False
-      | Some a => P a
-      end.
-  Proof.
-    destruct c'; simpl; crush.
-  Qed.
-  
-  
-  Lemma check_args_okP' c pl c'
-    : all_fresh c ->
-      List.fold_right
-        (fun t : pf =>
-           and
-             (forall c : named_list pf,
-                 all_fresh c -> (forall t0 : pf,(check_term_ok l c t t0) <->  (term_ok l c t t0))/\
-                                ((check_sort_ok l c t) <-> (sort_ok l c t))))
-        True pl ->
-      (check_args_ok l c pl c') <-> (args_ok l c pl c').
-  Proof.
-    intro frc.
-    revert c'.
-    induction pl; intro c'; cbn; crush.
-    {
-      destruct c'; intuition crush.
-      inversion H0.
-    }
-    {
-      intros; crush.
-      (*TODO: why does rewrite fail?
-      setoid_rewrite false_False.*)
-      rewrite TMP_match_list_to_bool.
-      crush.
-      apply peel_exists_iff; intro; crush.
-      apply peel_exists_iff; intro; crush.
-      apply and_iff_compat; crush.
-      crush.
-      (*TODO: get working?
-      rewrite rewrite_pair_let_to_proj *)
-      destruct e; crush.
-      rewrite TMP_match_option_to_bool.
-      crush.
-      apply peel_exists_iff; intro; crush.
-      apply and_iff_compat;
-        safe_specialize;
-        crush.
-      specialize (H c frc).
-      destruct H as [H H'].
-      crush.
-      specialize (H e); crush.
-    }
-  Qed.
-
-  
-  Lemma rewrite_if_eq_some A (a : A) (b : bool) c
-    : (if b then c else None) = Some a <-> (c = Some a) /\ b.
-  Proof.
-    destruct b; simpl; intuition crush.
-  Qed.
-  Hint Rewrite rewrite_if_eq_some : bool_utils.
-
-  
-  Lemma invert_term_ok_ax c n pfs t'
-    : term_ok l c (ax n pfs) t' <->
-      exists r, (n, r) \in l /\
-                           match r with
-                           | term_le_pf c' _ _ t =>
-                             is_dom (pf_subst (with_names_from c' pfs) t) t' /\
-                             args_ok l c pfs c'
-                           | _ => False
-                           end.
-  Proof.
-    intuition crush; inversion H; clear H; subst.
-    exists (term_le_pf c' e1 e2 t); intuition; crush.
-    destruct x; crush.
-  Qed.
-  Hint Rewrite invert_term_ok_ax : pfcore.
-
-  
-  Lemma invert_sort_ok_ax c n pfs
-    : sort_ok l c (ax n pfs) <->
-      exists r, (n, r) \in l /\
-                           match r with
-                           | sort_le_pf c' _ _ =>
-                             args_ok l c pfs c'
-                           | _ => False
-                           end.
-  Proof.
-    intuition crush; inversion H; clear H; subst.
-    exists (sort_le_pf c' t1 t2); intuition; crush.
-    destruct x; crush.
-  Qed.
-  Hint Rewrite invert_sort_ok_ax : pfcore.
-
-  Lemma invert_term_ok_sym c e t
-    : term_ok l c (sym e) t <-> term_ok l c e t.
-  Proof.
-    intuition crush; inversion H; crush.
-  Qed.
-  Hint Rewrite invert_term_ok_sym : pfcore.
-  
-  Lemma invert_sort_ok_sym c t
-    : sort_ok l c (sym t) <-> sort_ok l c t.
-  Proof.
-    intuition crush; inversion H; crush.
-  Qed.
-  Hint Rewrite invert_sort_ok_sym : pfcore.
-
-  Lemma invert_term_ok_trans c e1 e2 t
-    : term_ok l c (trans e1 e2) t <->
-      (term_ok l c e1 t /\
-       term_ok l c e2 t /\
-      exists e, is_codom e1 e /\ is_dom e2 e).
-  Proof.
-    intuition crush;
-    inversion H; crush.
-  Qed.
-  Hint Rewrite invert_term_ok_trans : pfcore.
-
-  
-  Lemma invert_sort_ok_trans c t1 t2
-    : sort_ok l c (trans t1 t2) <->
-      (sort_ok l c t1 /\
-       sort_ok l c t2 /\
-      exists t, is_codom t1 t /\ is_dom t2 t).
-  Proof.
-    intuition crush;
-    inversion H; crush.
-  Qed.
-  Hint Rewrite invert_sort_ok_trans : pfcore.
-
-  
-  Lemma invert_sort_ok_conv c pt p
-    : sort_ok l c (conv pt p) <-> False.
- Proof.
-    intuition crush;
-    inversion H; crush.
-  Qed.
-  Hint Rewrite invert_sort_ok_conv : pfcore.
-  
-  Lemma rewrite_exists_snd_determined_from_injectivity A B (f : A -> B) P x
-    : injective f -> (exists e : A, P e /\ f e = f x) <-> P x.
-  Proof.
-    intros ?.
-    firstorder crush.
-  Qed.
-  Hint Rewrite rewrite_exists_snd_determined_from_injectivity : bool_utils.
-
-  Lemma fold_eq_pf p1 p2 : eq_pf p1 p2 = (p1 == p2).
-  Proof.
-    reflexivity.
-  Qed.
-  Hint Rewrite fold_eq_pf : pfcore.
-  
-  Lemma check_okP c e
-    : all_fresh c ->
-      (forall t, check_term_ok l c e t <-> term_ok l c e t)
-        /\ (check_sort_ok l c e <-> sort_ok l c e).
-  Proof.
-    revert c.
-    induction e; intros c cfr; split;
-      cbn;intros; crush; simpl; crush.  (*TODO: figure out why simpl *)
-    {
-      apply peel_exists_iff; intro; crush.
-      apply and_iff_compat; crush.
-      destruct e; simpl; crush.
-      rewrite check_args_okP'; crush.
-    }
-    {
-      rewrite TMP_match_option_to_bool; crush.
-      apply peel_exists_iff; intro; crush.
-      apply and_iff_compat; crush.
-      destruct e; crush.
-      rewrite check_args_okP'; crush.
-    }
-    {                      
-      apply peel_exists_iff; intro; crush.
-      apply and_iff_compat; crush.
-      destruct e; crush.
-      rewrite check_args_okP'; crush.
-    }
-    {
-      rewrite TMP_match_option_to_bool; crush.
-      apply peel_exists_iff; intro; crush.
-      apply and_iff_compat; crush.
-      destruct e; crush.
-      rewrite check_args_okP'; crush.
-    }
-    {
-      unfold check_term_ok in *.
-      specialize (IHe c cfr); destruct IHe as [IHe1 IHe2].
-      specialize (IHe1 t); crush.
-    }
-    {
-      specialize (IHe c cfr); destruct IHe as [IHe1 IHe2]; crush.
-    }
-    {
-      etransitivity.
-      apply peel_exists_iff; intro.
-      apply and_iff_compat.
-      specialize (IHe1 c cfr); destruct IHe1 as [IHe11 IHe12].
-      specialize (IHe11 e); unfold check_term_ok in *; prepare_crush.
-      rewrite IHe11; crush.
-      prepare_crush.
-      apply peel_exists_iff; intro.
-      apply and_iff_compat.
-      specialize (IHe2 c cfr); destruct IHe2 as [IHe21 IHe22].
-      specialize (IHe21 e0); unfold check_term_ok in *; prepare_crush.
-      rewrite IHe21; crush.
-      prepare_crush.
-      apply peel_exists_iff; intro.
-      apply and_iff_compat.
-      rewrite rewrite_codom_eq; reflexivity.
-      prepare_crush.
-      apply peel_exists_iff; intro.
-      apply and_iff_compat.
-      rewrite rewrite_dom_eq; reflexivity.
-      rewrite rewrite_if_eq_some.
-      rewrite rewrite_if_eq_some.
-      reflexivity.
-      simpl.
-      intuition crush.
-      exists t; split; crush.
-      exists t; split; crush.
-      exists x; split; crush.
-      exists x; split; crush.
-    }
-  Admitted.    
-
-  Definition rewrite_term_okP c e (fr : all_fresh c) :=
-    proj1 (check_okP e fr).
-  Hint Rewrite rewrite_term_okP : pfcore.
-
-  Definition rewrite_sort_okP c e (fr : all_fresh c) :=
-    proj2 (check_okP e fr).
-  Hint Rewrite rewrite_sort_okP : pfcore.
-  
-  Lemma check_term_okP c e t
-    : all_fresh c ->
-      reflect (term_ok l c e t) (check_term_ok l c e t).
-  Proof using l_ok.
-    pose proof (@check_okP c e).
-    intuition.
-    eapply rewrite_reflect; [| apply idP].
-    rewrite H; reflexivity.
-  Qed.
-    
-  Lemma check_sort_okP c t
-      : all_fresh l ->
-        all_fresh c ->
-        reflect (sort_ok l c t) (check_sort_ok l c t).
-  Proof using l_ok.
-    pose proof (@check_okP c t).
-    intuition.
-    eapply rewrite_reflect; [| apply idP].
-    intuition.
-  Qed.
-  
-  Lemma ctx_ok_all_fresh c
-    : ctx_ok l c -> all_fresh c.
-  Proof using.
-    induction c; intro cok; inversion cok; subst; clear cok; break; simpl in *;
-      break_goal; auto.
-  Qed.
-  Hint Resolve ctx_ok_all_fresh : pfcore.
-
-  
-  Lemma check_ctx_okP c : reflect (ctx_ok l c) (check_ctx_ok l c).
-  Proof using l_ok.
-    induction c; intros; break; simpl; repeat constructor.
-    repeat lazymatch goal with
-           | [|- reflect _ (_&&_)]=>
-             (destruct_reflect_andb_l; simpl)
-           end.
-    lazymatch goal with
-    | [|- reflect _ ?p]=>
-      let H := fresh in my_case H p
-    end.
-    all: constructor.
-    {
-      constructor;
-      inversion IHc; auto.
-      apply /check_sort_okP; auto using ctx_ok_all_fresh with pfcore.
-    }
-    all: intro cok; inversion cok; subst; clear cok.
-      match goal with
-        [ H : reflect _ false |-_]=> inversion H
-      end; auto using ctx_ok_all_fresh.
-      {
-        rewrite <- rewrite_sort_okP in H4; eauto with pfcore.
-      }
-      eauto with pfcore.
-  Qed.
-
-  
-  Lemma rewrite_ctx_okP c : (check_ctx_ok l c) <-> (ctx_ok l c).
-  Proof using l_ok.
-    split.
-    - move /check_ctx_okP; auto.
-    - intros; apply /check_ctx_okP; auto.
-  Qed.
-  Hint Rewrite rewrite_ctx_okP : pfcore.
-  
-  Lemma invert_sort_rule_ok c args
-    : rule_ok l (sort_rule_pf c args) <-> ctx_ok l c /\ subseq args (map fst c).
-  Proof.
-    intuition ;inversion H; crush.
-  Qed.
-  Hint Rewrite invert_sort_rule_ok : pfcore.
-
-  
-  Lemma invert_term_rule_ok c args t
-    : rule_ok l (term_rule_pf c args t) <-> ctx_ok l c /\ subseq args (map fst c) /\ sort_ok l c t.
-  Proof.
-    intuition ;inversion H; crush.
-  Qed.
-  Hint Rewrite invert_term_rule_ok : pfcore.
-  
-  Lemma invert_sort_le_ok c t1 t2
-    : rule_ok l (sort_le_pf c t1 t2) <->
-      ctx_ok l c /\ sort_ok l c t1 /\ sort_ok l c t2 /\
-      is_exp t1 /\ is_exp t2.
-  Proof.
-    intuition;
-    inversion H; crush.
-  Qed.
-  Hint Rewrite invert_sort_le_ok : pfcore.
-
-  
-  Lemma invert_term_le_ok c e1 e2 t
-    : rule_ok l (term_le_pf c e1 e2 t) <->
-      ctx_ok l c /\ term_ok l c e1 t /\ term_ok l c e2 t /\ sort_ok l c t /\
-      is_exp e1 /\ is_exp e2 /\ is_exp t.
-  Proof.
-    intuition;
-    inversion H; crush.      
-  Qed.
-  Hint Rewrite invert_term_le_ok : pfcore.
-  
-  Lemma rewrite_rule_okP r : (check_rule_ok l r) <-> (rule_ok l r).
-  Proof using l_ok.
-    pose proof ctx_ok_all_fresh.
-    destruct r; intros; break; simpl.
-    all: intuition.
-    crush.
-    crush.
-    {
-      (*TODO: why does crush have an issue?*)
-      autorewrite with utils bool_utils in *;
-      intuition.
-      autorewrite with pfcore in *; eauto with pfcore.
-    }
-    {
-      (*TODO: why does crush have an issue?*)
-      autorewrite with utils bool_utils in *;
-      intuition;
-      autorewrite with pfcore in *; intuition; eauto with pfcore.
-      inversion H0; auto.
-    }
-    {
-      (*TODO: why does crush have an issue?*)
-      autorewrite with utils bool_utils in *;
-      intuition;
-      autorewrite with pfcore in *; intuition; eauto with pfcore.
-    }
-    crush.
-    {
-      (*TODO: why does crush have an issue?*)
-      autorewrite with utils bool_utils in *;
-      intuition;
-      autorewrite with pfcore in *; intuition; eauto with pfcore.
-    }
-    {
-      my_case H' (check_ctx_ok l n); simpl;
-      crush; intuition crush.
-      move: H' => /negP.
-      crush.
-    }
-  Qed.
-  Hint Rewrite rewrite_rule_okP : pfcore.
-  
-  
-  Lemma check_rule_okP r : reflect (rule_ok l r) (check_rule_ok l r).
-  Proof using l_ok.
-    reflect_from_iff rewrite_rule_okP.
-  Qed.
-  *)
-  
-End TermsAndRules.
+Lemma wf_lang_all_fresh l : wf_lang l -> all_fresh l.
+Proof.
+  induction l; break; simpl in *;
+    intro H; inversion H; subst; break_goal; auto.
+Qed.
 Hint Resolve wf_lang_all_fresh : pfcore.
+  
 
-(*TODO: pull crush out of section*)
+(*TODO: move to PfCore*)
+Lemma invert_wf_lang_cons l r n
+  : wf_lang ((n,r)::l) <-> wf_lang l /\ wf_rule l r /\ fresh n l.
+Proof.  
+  intuition; try inversion H; eauto with pfcore.
+Qed.
+Hint Rewrite invert_wf_lang_cons : pfcore.
 
-(*
-Lemma check_lang_ok_all_fresh l : check_lang_ok l -> all_fresh l.
+
+Lemma invert_wf_rule_sort l c args
+  : wf_rule l (Pf.wf_sort_rule c args) <-> wf_ctx l c /\ subseq args (map fst c).
+Proof.  
+  intuition; try inversion H; eauto with pfcore.
+Qed.
+Hint Rewrite invert_wf_rule_sort : pfcore.
+
+Lemma invert_wf_rule_term l c args t
+  : wf_rule l (Pf.wf_term_rule c args t) <-> wf_ctx l c /\ wf_sort l c t /\ subseq args (map fst c).
+Proof.  
+  intuition; try inversion H; eauto with pfcore.
+Qed.
+Hint Rewrite invert_wf_rule_term : pfcore.
+
+Lemma invert_wf_rule_le_sort l c t1 t2
+  : wf_rule l (Pf.wf_sort_le c t1 t2) <-> wf_ctx l c /\ wf_sort l c t1 /\ wf_sort l c t2.
+Proof.  
+  intuition; try inversion H; eauto with pfcore.
+Qed.
+Hint Rewrite invert_wf_rule_le_sort : pfcore.
+
+Lemma invert_wf_rule_le_term l c t e1 e2
+  : wf_rule l (Pf.wf_term_le c e1 e2 t) <->
+    wf_ctx l c /\ wf_sort l c t /\ wf_term l c e1 t /\ wf_term l c e2 t.
+Proof.  intuition; try inversion H; eauto with pfcore. Qed.
+Hint Rewrite invert_wf_rule_le_term : pfcore.
+
+Lemma invert_rule_eq_sort_term c args c' args' t'
+  : Pf.wf_sort_rule c args = Pf.wf_term_rule c' args' t' <-> False.
+Proof.  intuition; try inversion H; eauto with pfcore. Qed.
+Hint Rewrite invert_rule_eq_sort_term : pfcore.
+
+
+Lemma invert_rule_eq_sort_le_term c t1 t2 c' args' t'
+  : Pf.wf_sort_le c t1 t2 = Pf.wf_term_rule c' args' t' <-> False.
+Proof.  intuition; try inversion H; eauto with pfcore. Qed.
+Hint Rewrite invert_rule_eq_sort_le_term : pfcore.
+
+Lemma invert_rule_eq_sort_le_sort c t1 t2 c' args'
+  : Pf.wf_sort_le c t1 t2 = Pf.wf_sort_rule c' args' <-> False.
+Proof.  intuition; try inversion H; eauto with pfcore. Qed.
+Hint Rewrite invert_rule_eq_sort_le_sort : pfcore.
+
+Lemma invert_rule_eq_sort_le_term_le c t1 t2 c' t' e1' e2'
+  : Pf.wf_sort_le c t1 t2 = Pf.wf_term_le c' t' e1' e2' <-> False.
+Proof.  intuition; try inversion H; eauto with pfcore. Qed.
+Hint Rewrite invert_rule_eq_sort_le_term_le : pfcore.
+
+Lemma invert_rule_eq_sort_le c t1 t2 c' t1' t2'
+  : Pf.wf_sort_le c t1 t2 = Pf.wf_sort_le c' t1' t2' <-> c = c' /\ t1 = t1' /\ t2 = t2'.
+Proof. intuition; try inversion H; repeat f_equal; eauto with pfcore. Qed.
+Hint Rewrite invert_rule_eq_sort_le : pfcore.
+
+
+Lemma invert_rule_eq_term_le_term c e1 e2 t c' args' t'
+  : Pf.wf_term_le c e1 e2 t = Pf.wf_term_rule c' args' t' <-> False.
+Proof.  intuition; try inversion H; eauto with pfcore. Qed.
+Hint Rewrite invert_rule_eq_term_le_term : pfcore.
+
+Lemma invert_rule_eq_term_le_sort c e1 e2 t c' args'
+  : Pf.wf_term_le c e1 e2 t = Pf.wf_sort_rule c' args' <-> False.
+Proof. intuition; try inversion H; eauto with pfcore. Qed.
+Hint Rewrite invert_rule_eq_term_le_sort : pfcore.
+
+Lemma invert_rule_eq_term_le_sort_le c e1 e2 t c' t1' t2'
+  : Pf.wf_term_le c e1 e2 t = Pf.wf_sort_le c' t1' t2' <-> False.
+Proof.  intuition; try inversion H; eauto with pfcore. Qed.
+Hint Rewrite invert_rule_eq_term_le_sort_le : pfcore.
+
+Lemma invert_rule_eq_term_le c e1 e2 t c' e1' e2' t'
+  : Pf.wf_term_le c e1 e2 t = Pf.wf_term_le c' e1' e2' t'
+    <-> c = c' /\ t = t' /\ e1 = e1' /\ e2 = e2'.
+Proof. intuition; try inversion H; repeat f_equal; eauto with pfcore. Qed.
+Hint Rewrite invert_rule_eq_term_le : pfcore.
+
+Ltac pfcore_crush :=
+  repeat (simpl; autorewrite with utils bool_utils pfcore in *; intuition (subst; eauto with pfcore)).
+
+Local Lemma lang_mono l name r
+  : (forall c p t1 t2,
+        le_sort l c p t1 t2 ->
+        le_sort ((name,r)::l) c p t1 t2)
+    /\ (forall c p t e1 e2,
+           le_term l c p t e1 e2 ->
+           le_term ((name,r)::l) c p t e1 e2)
+    /\ (forall c c' pfs s1 s2,
+           le_subst l c c' pfs s1 s2 ->
+           le_subst ((name,r)::l) c c' pfs s1 s2)
+    /\ (forall c t,
+           wf_sort l c t ->
+           wf_sort ((name,r)::l) c t)
+    /\ (forall c e t,
+           wf_term l c e t ->
+           wf_term ((name,r)::l) c e t)
+    /\ (forall c s c',
+           wf_args l c s c' ->
+           wf_args ((name,r)::l) c s c')
+    /\ (forall c,
+           wf_ctx l c ->
+           wf_ctx ((name,r)::l) c).
 Proof using.
-  induction l; intros; repeat (break; simpl in * ); break_goal; auto.
-Qed.
-Hint Resolve check_lang_ok_all_fresh : pfcore.
-
-Lemma rewrite_lang_okP l : check_lang_ok l <-> lang_ok l.
-Proof.
-  induction l; intros; break; simpl.
-  split; eauto with pfcore.
-  autorewrite with bool_utils.
-  rewrite IHl.
-  intuition.
-  {
-    constructor; eauto.
-    unfold fresh; autorewrite with bool_utils; auto.
-    apply /check_rule_okP; auto.
-  }
-  all: inversion H1; subst; auto.
-  apply /check_rule_okP; auto.
+  apply judge_ind;
+    intros;
+    econstructor;
+    pfcore_crush.
 Qed.
 
-Lemma check_lang_okP l : reflect (lang_ok l) (check_lang_ok l).
-Proof using.
-    reflect_from_iff rewrite_lang_okP.
+Definition le_sort_lang_monotonicity l name r
+  := proj1 (lang_mono l name r).
+#[export] Hint Resolve le_sort_lang_monotonicity : pfcore.
+
+Definition le_term_lang_monotonicity l name r
+  := proj1 (proj2 (lang_mono l name r)).
+#[export] Hint Resolve le_term_lang_monotonicity : pfcore.
+
+Definition le_subst_lang_monotonicity l name r
+  := proj1 (proj2 (proj2 (lang_mono l name r))).
+#[export] Hint Resolve le_subst_lang_monotonicity : pfcore.
+
+Definition wf_sort_lang_monotonicity l name r
+  := proj1 (proj2 (proj2 (proj2 (lang_mono l name r)))).
+#[export] Hint Resolve wf_sort_lang_monotonicity : pfcore.
+
+Definition wf_term_lang_monotonicity l name r
+  := proj1 (proj2 (proj2 (proj2 (proj2 (lang_mono l name r))))).
+#[export] Hint Resolve wf_term_lang_monotonicity : pfcore.
+
+Definition wf_args_lang_monotonicity l name r
+  := proj1 (proj2 (proj2 (proj2 (proj2 (proj2 (lang_mono l name r)))))).
+#[export] Hint Resolve wf_args_lang_monotonicity : pfcore.
+
+Definition wf_ctx_lang_monotonicity l name r
+  := proj2 (proj2 (proj2 (proj2 (proj2 (proj2 (lang_mono l name r)))))).
+#[export] Hint Resolve wf_ctx_lang_monotonicity : pfcore.
+
+Lemma wf_rule_lang_monotonicity l name r' r
+  : wf_rule l r -> wf_rule ((name, r') :: l) r.
+Proof.
+  inversion 1; pfcore_crush.
 Qed.
-  
+#[export] Hint Resolve wf_rule_lang_monotonicity : pfcore.
 
-Ltac destruct_is_dom e :=
-      destruct e; intros;
-      [ eapply dom_var
-      | eapply dom_con
-      | eapply dom_ax_sort
-      | eapply dom_ax_term
-      | eapply dom_sym
-      | eapply dom_trans
-      | eapply dom_conv].
-Ltac destruct_is_codom e :=
-      destruct e; intros;
-      [ eapply codom_var
-      | eapply codom_con
-      | eapply codom_ax_sort
-      | eapply codom_ax_term
-      | eapply codom_sym
-      | eapply codom_trans
-      | eapply codom_conv].
-
-Lemma is_dom_monotonicity t t' n r l
-  : is_dom l t t' -> is_dom ((n,r)::l) t t'
-with is_codom_monotonicity t t' n r l
-     : is_codom l t t' -> is_codom ((n,r)::l) t t'.
-Proof.
-    
-    all:intro d; first [destruct_is_dom d | destruct_is_codom d];
-      repeat match goal with
-             |[H : List.Forall2 _ _ _ |-_]=>
-              induction H; constructor; eauto
-            |[|- is_true (_ \in _::_)]=>
-             rewrite in_cons; apply /orP; right; eauto
-             end; eauto.
-Qed.
-
-
-Ltac destruct_term_ok e :=
-  destruct e; intros;
-  [ eapply term_ok_ax
-  | eapply term_ok_con
-  | eapply term_ok_trans
-  | eapply term_ok_sym
-  | try eapply term_ok_var
-  | eapply term_ok_conv].
-
-
-Ltac destruct_sort_ok s :=
-  destruct s; intros;
-  [ eapply sort_ok_ax
-  | eapply sort_ok_con
-  | eapply sort_ok_trans
-  | eapply sort_ok_sym].
-
-
-Ltac destruct_args_ok s :=
-  destruct s; intros;
-  [ eapply args_ok_nil
-  | eapply args_ok_cons].
-
-Fixpoint sort_lang_monotonicity l c t name r
-     (les : sort_ok l c t) {struct les}
-     : sort_ok ((name,r)::l) c t
-with term_lang_monotonicity l c e t name r
-     (letm: term_ok l c e t) {struct letm}
-     : term_ok ((name,r)::l) c e t
-with args_lang_monotonicity l c al c' name r
-     (lea : args_ok l c al c') {struct lea}
-     : args_ok ((name,r)::l) c al c'.
-Proof.
-  {
-    destruct_sort_ok les; 
-      repeat match goal with
-             |[|- is_true (_ \in _::_)]=>
-              rewrite in_cons; apply /orP; right; eauto
-             end; eauto using is_dom_monotonicity, is_codom_monotonicity.
-  }
-  {
-      destruct_term_ok letm;
-      repeat match goal with
-             |[|- is_true (_ \in _::_)]=>
-              rewrite in_cons; apply /orP; right; eauto
-             end; eauto using is_dom_monotonicity, is_codom_monotonicity.
-  }
-  {
-    destruct_args_ok lea; eauto using is_dom_monotonicity.
-  }
-Qed.
-
-(*TODO: move to pf.v*)
-Lemma pf_subst_nil p : pf_subst [::] p = p.
-Proof.
-  induction p; simpl; auto.
-  { revert H; induction l; intros; simpl in *; break; simpl in *; auto.
-    f_equal; f_equal; auto.
-    pose proof (IHl H0) as H'; inversion H'.
-    rewrite H2.
-    assumption.
-  }
-  { revert H; induction pfs; intros; simpl in *; break; simpl in *; auto.
-    f_equal; f_equal; auto.
-    pose proof (IHpfs H0) as H'; inversion H'.
-    rewrite H2.
-    assumption.
-  }
-  {
-    rewrite IHp; reflexivity.
-  }
-  {
-    rewrite IHp1 IHp2; reflexivity.
-  }
-  {
-    rewrite IHp1 IHp2; reflexivity.
-  }
-Qed.
-
-Lemma map_pf_subst_nil pl : map (pf_subst [::]) pl = pl.
-Proof.
-  induction pl; simpl; rewrite ?pf_subst_nil; f_equal; auto.
-Qed.
-
-(*TODO: move to Pf*)
-(*TODO: requires wfness or altered definition; can't have both the
-  above and below thms
- *)
-
-Inductive ws_pf {c : list string} : pf -> Prop :=
-| ws_var x : x \in c -> ws_pf (pvar x)
-| ws_con n l : List.Forall ws_pf l -> ws_pf (pcon n l)
-| ws_ax n l : List.Forall ws_pf l -> ws_pf (ax n l)
-| ws_sym p : ws_pf p -> ws_pf (sym p)
-| ws_trans p1 p2 : ws_pf p1 -> ws_pf p2 -> ws_pf (trans p1 p2)
-| ws_conv p1 p2 : ws_pf p1 -> ws_pf p2 -> ws_pf (conv p1 p2).
-
-Arguments ws_pf : clear implicits.
-
-Lemma pf_subst_lookup s s' n
-  : n \in (map fst s') ->
-    pf_subst s (named_list_lookup (pvar n) s' n)
-    = named_list_lookup (pvar n) (named_map (pf_subst s) s') n.
-Proof.
-  induction s'; simpl; [easy |].
-  rewrite in_cons.
-  break; simpl in *.
-  change (n =? s0)%string with (n == s0).
-  case neq: (n == s0); simpl; auto.
-Qed.        
-
-Lemma pf_subst_distributes s s' p
-  : ws_pf (map fst s') p ->
-    pf_subst s (pf_subst s' p)
-    = pf_subst (named_map (pf_subst s) s') p.
-Proof.
-  induction p; intro wsp; inversion wsp; subst; clear wsp; simpl.
-  by apply pf_subst_lookup.
-  1,2: match goal with
-         [l : seq pf |- _]=>
-         revert dependent l; intro l; induction l; simpl; intros;
-           f_equal; f_equal;
-             match goal with
-             | [H : List.Forall _ (_::_)|-_] => inversion H; clear H; subst
-             end;
-             intuition;
-             match goal with
-             | [H : pcon _ _ = pcon _ _ |-_] => inversion H; clear H; subst
-             | [H : ax _ _ = ax _ _ |-_] => inversion H; clear H; subst
-             end; auto
-       end.
-  all:intuition; f_equal; auto.
-Qed.
-
-    
-
-Lemma named_map_with_names_from {A B C:Set} (f : A -> B) (c : named_list C) s
-  : named_map f (with_names_from c s)
-    = with_names_from c (map f s).
-Proof.
-  revert c; induction s; intro c; destruct c; break; simpl; auto.
-  f_equal; eauto.
-Qed.
-
-
-Lemma is_dom_unique l p p1 p2
-  : lang_ok l -> is_dom l p p1 -> is_dom l p p2 -> p1 = p2.
-Proof.
-  intro lok.
-  move /(is_domP lok) /eqP => d1.
-  move /(is_domP lok) /eqP => d2.
-  congruence.
-Qed.
-
-Lemma is_codom_unique l p p1 p2
-  : lang_ok l -> is_codom l p p1 -> is_codom l p p2 -> p1 = p2.
-Proof.
-  intro lok.
-  move /(is_codomP lok) /eqP => d1.
-  move /(is_codomP lok) /eqP => d2.
-  congruence.
-Qed.
-  
-Lemma is_dom_and_codom_subst_monotonicity l tc t td sc s sd
-  : is_dom l t td -> is_codom l t tc ->
-    List.Forall2 (fun p1 p2 => p1.1 = p2.1 /\ is_codom l p1.2 p2.2) s sc ->
-    List.Forall2 (fun p1 p2 => p1.1 = p2.1 /\ is_dom l p1.2 p2.2) s sd ->
-    (is_dom l (pf_subst s t) (pf_subst sd td)
-     /\ is_codom l (pf_subst s t) (pf_subst sc tc)).
-Proof.
-  revert tc td s sc sd;
-    induction t; intros tc td s.
-  {
-    induction s; intros sc sd is_d is_c allc alld;
-      inversion allc; inversion alld; clear allc; clear alld;
-        break;simpl in *; subst; rewrite ?pf_subst_nil; auto;
-          inversion is_d; inversion is_c; clear is_d is_c; subst.
-    inversion H; inversion H4; subst; clear H H4.
-    simpl; case_match; auto.
-    apply IHs; eauto; constructor.
-  }
-  {
-    intros sc sd is_d is_c allc alld;
-      inversion is_c; inversion is_d; clear is_c is_d;
-      break;simpl in *; subst.
-    revert pl_r pl_l H H7 H3; induction l0; simpl;
-      intros pl_r pl_l IH fl1 fl2; inversion fl1; inversion fl2; clear fl1 fl2;
-        subst; simpl; repeat constructor;
-      break;
-      try eapply H; eauto;
-      specialize IHl0 with l'0 l';
-      specialize (IHl0 H0 H3 H8);
-      destruct IHl0 as [IHd IHc].
-      by inversion IHd.
-      by inversion IHc.
-  }
-  {
-    intros sc sd is_d is_c allc alld;
-      inversion is_c; inversion is_d; clear is_c is_d;
-      break;simpl in *; subst.
-
-    rewrite !pf_subst_distributes.
-    rewrite !named_map_with_names_from.    
-    
-    revert pl_r pl_l H H7 H2; induction pfs; simpl;
-      intros pl_r pl_l IH fl1 fl2; inversion fl1; inversion fl2; clear fl1 fl2;
-        subst; simpl;
-          (split; [eapply dom_ax_sort | eapply codom_ax_sort]); try constructor;
-            intuition; try eapply H; eauto.
-    admit (*TODO: forall from fold_right; induction not strong enough*).
-    admit.
-    (*TODO: need ws assumptions*)    
-Admitted.
-
-  
-Lemma is_dom_subst_monotonicity l t t' s s'
-  : is_dom l t t' -> List.Forall2 (fun p1 p2 => p1.1 = p2.1 /\ is_dom l p1.2 p2.2) s s' -> is_dom l (pf_subst s t) (pf_subst s' t').
-Proof.
-  (*TODO: show dom/codom always exist, use w/ above to prove this*)
-Admitted.
-  
-Lemma is_codom_subst_monotonicity l t t' s s'
-     : is_codom l t t' -> List.Forall2 (fun p1 p2 => p1.1 = p2.1 /\ is_codom l p1.2 p2.2) s s' -> is_codom l (pf_subst s t) (pf_subst s' t').
-Proof.
-  (*TODO: show dom/codom always exist, use w/ above to prove this*)
-Admitted.
-
-
-(*TODO: move to utils*)
-(*redefined to use the right concatenation*)
-Definition flat_map {A B} (f : A -> list B) :=
-  fix flat_map l :=
-  match l with
-  | [::] => [::]
-  | x :: t => (f x ++ flat_map t)
-  end.
-
-(*TODO: move to Pf*)
-Fixpoint fv (p : pf) :=
-  match p with
-  | pvar x => [:: x]
-  | pcon _ l => flat_map fv l
-  | ax _ l => flat_map fv l
-  | sym p => fv p
-  | trans p1 p2 => fv p1 ++ fv p2
-  | conv p1 p2 => fv p1 ++ fv p2
-  end.
-
-
-
-Lemma fv_term_ok l c e t
-  : term_ok l c e t ->
-    included (fv e) (map fst c)
-with fv_args_ok l c s c'
-     : args_ok l c s c' ->
-       included (flat_map fv s) (map fst c)
-with fv_sort_ok l c t
-  : sort_ok l c t ->
-    included (fv t) (map fst c).
-Proof.
-  {
-    intro tok; inversion tok; clear tok; subst; simpl;
-      first [eapply fv_args_ok; eauto
-            | rewrite included_app; apply /andP; split; eauto
-            | eauto].
-    rewrite Bool.andb_true_r.
-    eapply pair_fst_in; eauto.
-  }
-  {
-    intro tok; inversion tok; clear tok; subst; simpl;
-      first [eapply fv_args_ok; eauto
-            | rewrite included_app; apply /andP; split; eauto
-            | eauto].
-  }
-  {
-    intro tok; inversion tok; clear tok; subst; simpl;
-      first [eapply fv_args_ok; eauto
-            | rewrite included_app; apply /andP; split; eauto
-            | eauto].
-  }
-Qed.
-
-(* Will later be able to prove this by appealing to the fact that 
-   sort in an ok ctx are ok, but we need monotonicity facts first
-   so we prove this directly here.
-*)
-Lemma fv_in_ctx l c n t
-  : ctx_ok l c ->
-    (n,t) \in c ->
-    included (fv t) (map fst c).
-Proof.
-  intro cok; induction cok; simpl; auto.
-  rewrite in_cons.
-  move /orP => [/eqP []|]; intros; subst.
-  {
-    apply included_rest.
-    eapply fv_sort_ok; eauto.
-  }
-  {
-    apply included_rest; eauto.
-  }
-Qed.
-
-Lemma strengthen_pf_subst t s name x
-  : name \notin (map fst s) ->
-    included (fv t) (map fst s) ->
-    pf_subst ((name, x)::s) t = pf_subst s t.
-Proof.
-  induction t; simpl; intros; try f_equal;
-    repeat match goal with
-           |[H : is_true (included (_++_) _)|-_] =>
-            rewrite included_app in H;
-              move: H => /andP []; intros
-           |[H : is_true (included (flat_map _ ?l) _)|-_] =>
-            revert dependent l; intro l; induction l; simpl; auto;
-              intuition; f_equal; eauto
-           end; eauto.
-  {
-    rewrite Bool.andb_true_r in H0.
-    change (n =? name)%string with (n == name).
-    my_case neq (n == name); auto.
-    move: neq => /eqP neq; subst.
-    rewrite H0 in H.
-    easy.
-  }
-Qed.
-
-Lemma subst_ok_names_eq l c s c'
-  : subst_ok l c s c' -> [seq i.1 | i <- s] = [seq i.1 | i <- c'].
-Proof.
-  induction 1; simpl in *; f_equal; eauto.
-Qed.
-
-Lemma term_ok_lookup l c' s c t x
-  : lang_ok l ->
-    ctx_ok l c ->
-    subst_ok l c' s c ->
-    (x,t) \in c ->
-    forall t',
-    is_dom l (pf_subst s t) t' ->
-    term_ok l c' (named_list_lookup (pvar x) s x) t'.
-Proof.
-  intros lok allf.
-  induction 1; simpl in *; break; try easy.
-  rewrite in_cons.
-  cbn.
-  inversion allf; clear allf; subst.
-  case xeq: (x =? name)%string; simpl; [move: xeq => /eqP xeq; subst|].
-  {
-    change (eq_pf t t0) with (t == t0).
-    case teq: (t == t0); [move: teq => /eqP teq; subst|];
-      intros ? t'0.
-    {
-      replace (pf_subst ((name,e)::s) t0) with (pf_subst s t0).
-      intro isd.
-      pose proof (is_dom_unique lok H0 isd); subst; auto.
-      symmetry; apply strengthen_pf_subst;
-        erewrite subst_ok_names_eq; eauto.
-      eapply fv_sort_ok; eauto.
-    }
-    {
-      simpl in *.
-      apply pair_fst_in in H2.
-      rewrite H2 in H5.
-      easy.
-    }
-  }
-  {
-    intros tin t'0.
-    rewrite strengthen_pf_subst; eauto;
-      erewrite subst_ok_names_eq; eauto.
-      eapply fv_in_ctx; eauto.
-  }
-Qed.
-
-
-Lemma Forall2_pair_from_maps A B P Q (l1 l2 : list (A*B))
-  : List.Forall2 P (map fst l1) (map fst l2) ->
-    List.Forall2 Q (map snd l1) (map snd l2) ->
-    List.Forall2 (fun p1 p2 => P p1.1 p2.1 /\ Q p1.2 p2.2) l1 l2.
-Proof.
-  revert l2; induction l1; intro l2; destruct l2;
-    break;
-    simpl;
-    intro lfp; inversion lfp;
-      intro lfq; inversion lfq;
-        subst;auto.
-Qed.
-
-
-Lemma Forall2_eq_refl A (lst : list A) : List.Forall2 eq lst lst.
-Proof.
-  induction lst; simpl; eauto.
-Qed.
-
-(* TODO: move to utils? need more general types to do so*)
-Lemma map_fst_with_names_from (A B:Set) (c:named_list_set A) (s : list B)
-  : size s = size c -> map fst (with_names_from c s) = map fst c.
-Proof using .
-  elim: c s; intros until s; case: s; intros; break;simpl in *; auto.
-  { inversion H0. }
-  {
-    f_equal; auto.
-  }
-Qed.
-
-
-Lemma map_snd_with_names_from (A B:Set) (c:named_list_set A) (s : list B)
-  : size s = size c -> map snd (with_names_from c s) = s.
-Proof using .
-  elim: c s; intros until s; case: s; intros; break;simpl in *; auto.
-  { inversion H. }
-  {
-    f_equal; auto.
-  }
-Qed.
-
-
-Lemma is_dom_codom_exists_sort l c p
-  : sort_ok l c p ->
-    (exists p', is_dom l p p') /\
-    (exists p', is_codom l p p')
-with is_dom_codom_exists_term l c p t
-  : term_ok l c p t ->
-    (exists p', is_dom l p p') /\
-    (exists p', is_codom l p p').
-Proof.
-Admitted.
-
-Lemma is_dom_codom_exists_args l c pfs c'
-  : args_ok l c pfs c' ->
-    (exists p', List.Forall2 (is_dom l) pfs p') /\
-    (exists p', List.Forall2 (is_codom l) pfs p').
-Proof.
-  induction 1; simpl; firstorder.
-  eexists; constructor; eauto with pfcore.
-  eexists; constructor; eauto with pfcore.
-  destruct (is_dom_codom_exists_term H1); firstorder.
-  eauto.
-  destruct (is_dom_codom_exists_term H1); firstorder.
-  eauto.
-Qed.
-
-
-Lemma with_names_from_subst_ok l c s c'
-  : subst_ok l c s c' -> map fst s = map fst c'.
-Proof.
-  induction 1; break; simpl; f_equal; eauto.
-Qed.
-
-Lemma subst_ok_args_ok l c s c'
-  : subst_ok l c s c' -> args_ok l c (map snd s) c'.
-Proof.
-  induction 1; simpl; eauto with pfcore.
-  econstructor; eauto with pfcore.
-  replace (with_names_from c' (map snd s)) with s; auto.
-    
-  erewrite with_names_from_names_eq.
-  symmetry.
-  apply with_names_from_snd.
-  symmetry; eapply with_names_from_subst_ok; eauto.
-Qed.
-Hint Resolve subst_ok_args_ok.  
-
-(*TODO: figure out which ctxs need to be ok (could be all)
-*)
-Lemma sort_subst_monotonicity l c t c' s
-  : sort_ok l c t -> ctx_ok l c -> ctx_ok l c' ->
-    subst_ok l c' s c ->
-    sort_ok l c' (pf_subst s t)
-with term_subst_monotonicity l c e t c' s t'
-  : term_ok l c e t -> ctx_ok l c -> ctx_ok l c' ->
-    subst_ok l c' s c ->
-    is_dom l (pf_subst s t) t' ->
-    term_ok l c' (pf_subst s e) t'
-with args_subst_monotonicity l c ss c' s c''
-  : args_ok l c ss c' -> ctx_ok l c -> ctx_ok l c'' ->
-    subst_ok l c'' s c ->
-    args_ok l c'' (map (pf_subst s) ss) c'.
-Proof.
-  {
-    intros sok cok c'ok subok.
-    pose proof (is_dom_codom_exists_args (subst_ok_args_ok subok)).
-    revert cok c'ok subok H.
-    destruct sok; intuition.
-
-    {
-      eapply sort_ok_ax; eauto.
-    }
-    {
-      eapply sort_ok_con; eauto.
-    }
-    {
-      eapply sort_ok_trans; eauto; fold pf_subst.
-      known issue:
-        when applying a subst to a trans, need to project left or right out
-      alternatives/ideas:
-          embed l and r terms in ax to avoid lang in pf_subst
-          lean into non-canonical proofs, make pf_subst a constructor
-          may want to re-separate proof-terms
-    }
-    | eapply sort_ok_con | eapply sort_ok_trans | eapply sort_ok_sym ]
-    apply 
-    destruct_sort_ok sok; fold pf_subst;
-    eauto.
-        [ apply is_codom_subst_monotonicity; intuition; firstorder; eauto
-        | apply is_dom_subst_monotonicity; intuition; firstorder; eauto].
-      {
-        let x := open_constr:(with_names_from s _) in
-        instantiate (1:=x).
-        apply Forall2_pair_from_maps.
-        rewrite map_fst_with_names_from.
-        apply Forall2_eq_refl.
-        2: rewrite map_snd_with_names_from; eauto.
-        admit.
-        admit. (*TODO: size lemma*)
-      }
-      {
-        TODO: why the same x?
-        apply Forall2_pair_from_maps.
-        rewrite map_fst_with_names_from.
-        apply Forall2_eq_refl.
-        2: rewrite map_snd_with_names_from; eauto.
-        TODO: what is x0; 
-        admit.
-        admit. (*TODO: size lemma*)
-      }
-        
-    admit
-    (*TODO: need existence of dom/codom
-      for substitutions
-     *).
-    admit.
-  }
-  {
-    intro sok;
-    destruct_term_ok sok; fold pf_subst; simpl; eauto; cycle 4.
-    TODO: need lookup wfness lemma
-        
-      
-        [ apply is_codom_subst_monotonicity; eauto
-        | apply is_dom_subst_monotonicity; eauto].
-    admit
-    (*TODO: need existence of dom/codom
-      for substitutions
-     *).
-    admit.
-  }
-                                          
-    eapply args_subst_monotonicity.
-    repeat match goal with
-             |[|- is_true (_ \in _::_)]=>
-              rewrite in_cons; apply /orP; right; eauto
-             end; eauto using is_dom_monotonicity, is_codom_monotonicity.
-  }
-  {
-      destruct_term_ok letm;
-      repeat match goal with
-             |[|- is_true (_ \in _::_)]=>
-              rewrite in_cons; apply /orP; right; eauto
-             end; eauto using is_dom_monotonicity, is_codom_monotonicity.
-  }
-  {
-    destruct lea; constructor; eauto.
-  }
-Qed.
-*)
-
-
-(*TODO: prove!!!!!!!!!!!!!!!!!!!!!!!!!!*)
 Lemma rule_in_wf l r name
   : wf_lang l -> (name,r) \in l -> wf_rule l r.
+Proof.
+  induction 1; pfcore_crush.
+  (*TODO: why does regular rewrite fail?*)
+  setoid_rewrite pair_equal_spec in H3.
+  pfcore_crush.
+Qed.
+
+Lemma le_subst_subst_monotonicity l c c' c'' pfs s1 s2 pfs' s1' s2'
+  : le_subst l c' c'' pfs s1 s2 ->
+    le_subst l c c' pfs' s1' s2' ->
+    le_subst l c c'' (named_map (pf_subst pfs') pfs)
+             (named_map (wfexp_subst s1') s1)
+             (named_map (wfexp_subst s2') s2).
+Proof.
+  induction 1; pfcore_crush.
+  constructor; pfcore_crush.
+  (*
+    TODO: prove subst_assoc
+  rewrite wfexp_subst_assoc.
+  apply le_term_subst; pfcore_crush. *)
+Admitted.
+#[export] Hint Resolve le_subst_subst_monotonicity : pfcore.
+
+(*TODO: move to PfCoreDefs *)
+Scheme wf_sort_ind'' := Minimality for wf_sort Sort Prop
+  with wf_term_ind'' := Minimality for wf_term Sort Prop
+  with wf_args_ind'' := Minimality for wf_args Sort Prop.
+Combined Scheme wf_ind
+         from wf_sort_ind'', wf_term_ind'', wf_args_ind''.
+
+Local Lemma wf_subst_mono l c' s
+  : (forall c t,
+        wf_sort l c t ->
+        wf_subst l c' s c ->
+        wf_sort l c' (wfexp_subst s t))
+    /\ (forall c e t,
+           wf_term l c e t ->
+           wf_subst l c' s c ->
+           wf_term l c' (wfexp_subst s e) (wfexp_subst s t))
+    /\ (forall c s' c'',
+           wf_args l c s' c'' ->
+           wf_subst l c' s c ->
+           wf_args l c' (map (wfexp_subst s) s') c'').
+Proof using.
+  apply wf_ind;
+    intros;
+    try econstructor;
+    pfcore_crush.
+  (*
+    TODO: prove subst_assoc*)
 Admitted.
